backend/Tailcallproof.v
@@ -311,6 +311,17 @@ Proof.
   eapply (Genv.match_genvs_allowed_calls TRANSL). eauto.
 Qed.
 
+Lemma type_of_call_translated:
+  forall cp vf,
+    (* Val.lessdef vf vf' -> *)
+    (* Genv.find_funct ge vf = Some fd -> *)
+    Genv.allowed_call ge cp vf ->
+    Genv.type_of_call ge cp vf = Genv.type_of_call tge cp vf.
+Proof.
+  intros cp vf H.
+  eapply (Genv.match_genvs_type_of_call TRANSL). eauto.
+Qed.
+
 (* This part has been adapted from Inliningproof.v; perhaps everything can be
 generalized and unified. *)
 
@@ -621,6 +632,24 @@ Proof.
   eapply exec_Icall; eauto. apply sig_preserved.
   eapply find_function_ptr_translated; eauto.
   rewrite comp_transl. eapply allowed_call_translated; eauto.
+  rewrite <- E.
+  intros CROSS.
+  assert (forall rs rs',
+             regs_lessdef rs rs' ->
+             forall l,
+               Forall not_ptr rs ## l ->
+               Forall not_ptr rs' ## l).
+  { clear. intros rs rs' LESSDEF.
+    induction l; intros.
+    - eauto.
+    - inv H.
+      constructor.
+      + specialize (LESSDEF a). inv LESSDEF; eauto.
+        rewrite <- H0 in H2; now simpl in H2.
+      + eauto. }
+  eapply H1; eauto.
+  eapply NO_CROSS_PTR; eauto.
+  erewrite type_of_call_translated; eauto.
   constructor. constructor; auto.
     apply (cenv_compat_linkorder _ _ _ ORDER (compenv_program_compat _)).
   { easy. }
