backend/Unusedglobproof.v
@@ -1053,6 +1053,7 @@ Proof.
 
   intros (tvf & C & D).
   econstructor; split. eapply exec_Icall; eauto.
+  admit.
   econstructor; eauto.
   econstructor; eauto.
   change (Mem.valid_block m sp0). eapply Mem.valid_block_inject_1; eauto.
@@ -1157,7 +1158,7 @@ Proof.
   inv STACKS. econstructor; split.
   eapply exec_return.
   econstructor; eauto. apply set_reg_inject; auto.
-Qed.
+Admitted.
 
 (** Relating initial memory states *)
 
